Add litmus tests and refactor code.

LeanCats/Data.lean
@@ -18,11 +18,28 @@ structure Effect : Type where
   isFinalWrite : Bool
 deriving Inhabited, BEq, Repr, DecidableEq
 
+structure EventId where
+  id : Nat
+deriving DecidableEq
+
 structure Event where
   id : Nat   -- Unique identifier, consistent with program order for a given thread
   t_id : Nat      -- Thread ID
   effect : Effect -- Action performed
   tag : Σ tagType : Type, tagType
+
+-- Unsafe.
+axiom event_id_unique :
+  ∀ e₁ e₂ : Event, e₁.id = e₂.id -> e₁ = e₂
+
+instance : DecidableEq Event := by
+  intro a b
+  by_cases h : a.id = b.id
+  · exact isTrue (event_id_unique a b h)
+  · exact isFalse (by
+      intro hEq
+      have : a.id = b.id := by simp [hEq]
+      exact h this)
 
 instance : BEq Event where
   beq e1 e2 := e1.id == e2.id
@@ -44,6 +61,7 @@ inductive Normal where
 -- reads, gathered in the set R;
 -- branch events, gathered in the set B;
 -- fences, gathered in the set F.
+-- this is the base events, because the CandidateExecution needs to extends it.
 structure Events where
   (IW : Set Event)
   (R : Set Event)
@@ -51,36 +69,38 @@ structure Events where
   (B : Set Event)
   (F : Set Event)
   (RMW : Set Event)
-  (SRCU : Set Event)
   (M : Set Event)
 
-def Events.all (evts : Events) :=
-  evts.IW ∪ evts.R ∪ evts.W ∪ evts.B ∪ evts.F ∪ evts.RMW ∪ evts.SRCU ∪ evts.M
+@[simp] def Events.all (evts : Events) :=
+  evts.IW ∪ evts.R ∪ evts.W ∪ evts.B ∪ evts.F ∪ evts.RMW ∪ evts.M
 
 instance : Membership Event Events where
   mem := fun es e => e ∈ es.all
 
--- We can derive some relations based on the events.
-@[simp] def Events.rf (evts : Events) : SetRel Event Event :=
-  λ (w, r) =>
+@[simp] def Events.preCo (evts : Events) (co : SetRel Event Event) : Prop :=
+  ∀ e₁ e₂ : Event, (e₁, e₂) ∈ co ->
+    e₁ ∈ evts.all
+    ∧ e₂ ∈ evts.all
+    ∧ e₁.effect.op = Op.write
+    ∧ e₂.effect.op = Op.write
+    ∧ e₁.effect.location = e₂.effect.location
+
+class wellformed.co (evts : Events) (corel : SetRel Event Event) : Prop where
+  -- The Type is the Prop, and the proof is the term, do not use :=
+  irrefl : ∀ e : Event, ¬ (e, e) ∈ corel
+  trans : ∀ e₁ e₂ e₃, (e₁, e₂) ∈ corel -> (e₂, e₃) ∈ corel -> (e₁, e₃) ∈ corel
+  preco : evts.preCo corel
+
+@[simp] def wellformed.rf (evts : Events) (rf : SetRel Event Event) : Prop :=
+  ∀ (w r : Event), (w, r) ∈ rf ->
     w ∈ evts.W ∧ r ∈ evts.R
     ∧ w.effect.location = r.effect.location
-    ∧ r.effect.value = w.effect.value
     ∧ r.id ≠ w.id
 
 @[simp] def Events.po (evts : Events) : SetRel Event Event :=
   λ (a, b) =>
-    a ∈ evts ∧ b ∈ evts ∧ a.t_id = b.t_id ∧ a.id < b.id
+    a ∈ evts.all ∧ b ∈ evts.all ∧ a.t_id = b.t_id ∧ a.id < b.id
 
-/-
-In the definition of the cat specification, we know that the tag is just an id.
-Basically it's a event.
-
-What we want is a:
-  enum A = 'z | 'a
-  enum B = 'z | 'a
-  etc
-
--/
+#check trichotomous
 
 end Data
